\documentclass[11pt]{article}

% NOTE: Add in the relevant information to the commands below; or, if you'll be using the same information frequently, add these commands at the top of paolo-pset.tex file. 
\newcommand{\name}{AgustÃ­n Esteva}
\newcommand{\email}{aesteva@uchicago.edu}
\newcommand{\classnum}{270}
\newcommand{\subject}{Complex Variables}
\newcommand{\instructors}{Robert Fefferman}
\newcommand{\assignment}{Problem Set 2}
\newcommand{\semester}{Spring 2025}
\newcommand{\duedate}{4-17-2025}
\newcommand{\bA}{\mathbf{A}}
\newcommand{\bB}{\mathbf{B}}
\newcommand{\bC}{\mathbf{C}}
\newcommand{\bD}{\mathbf{D}}
\newcommand{\bE}{\mathbf{E}}
\newcommand{\bF}{\mathbf{F}}
\newcommand{\bG}{\mathbf{G}}
\newcommand{\bH}{\mathbf{H}}
\newcommand{\bI}{\mathbf{I}}
\newcommand{\bJ}{\mathbf{J}}
\newcommand{\bK}{\mathbf{K}}
\newcommand{\bL}{\mathbf{L}}
\newcommand{\bM}{\mathbf{M}}
\newcommand{\bN}{\mathbf{N}}
\newcommand{\bO}{\mathbf{O}}
\newcommand{\bP}{\mathbf{P}}
\newcommand{\bQ}{\mathbf{Q}}
\newcommand{\bR}{\mathbf{R}}
\newcommand{\bS}{\mathbf{S}}
\newcommand{\bT}{\mathbf{T}}
\newcommand{\bU}{\mathbf{U}}
\newcommand{\bV}{\mathbf{V}}
\newcommand{\bW}{\mathbf{W}}
\newcommand{\bX}{\mathbf{X}}
\newcommand{\bY}{\mathbf{Y}}
\newcommand{\bZ}{\mathbf{Z}}
\newcommand{\Vol}{\text{Vol}}

%% blackboard bold math capitals
\newcommand{\bbA}{\mathbb{A}}
\newcommand{\bbB}{\mathbb{B}}
\newcommand{\bbC}{\mathbb{C}}
\newcommand{\bbD}{\mathbb{D}}
\newcommand{\bbE}{\mathbb{E}}
\newcommand{\bbF}{\mathbb{F}}
\newcommand{\bbG}{\mathbb{G}}
\newcommand{\bbH}{\mathbb{H}}
\newcommand{\bbI}{\mathbb{I}}
\newcommand{\bbJ}{\mathbb{J}}
\newcommand{\bbK}{\mathbb{K}}
\newcommand{\bbL}{\mathbb{L}}
\newcommand{\bbM}{\mathbb{M}}
\newcommand{\bbN}{\mathbb{N}}
\newcommand{\bbO}{\mathbb{O}}
\newcommand{\bbP}{\mathbb{P}}
\newcommand{\bbQ}{\mathbb{Q}}
\newcommand{\bbR}{\mathbb{R}}
\newcommand{\bbS}{\mathbb{S}}
\newcommand{\bbT}{\mathbb{T}}
\newcommand{\bbU}{\mathbb{U}}
\newcommand{\bbV}{\mathbb{V}}
\newcommand{\bbW}{\mathbb{W}}
\newcommand{\bbX}{\mathbb{X}}
\newcommand{\bbY}{\mathbb{Y}}
\newcommand{\bbZ}{\mathbb{Z}}

%% script math capitals
\newcommand{\sA}{\mathscr{A}}
\newcommand{\sB}{\mathscr{B}}
\newcommand{\sC}{\mathscr{C}}
\newcommand{\sD}{\mathscr{D}}
\newcommand{\sE}{\mathscr{E}}
\newcommand{\sF}{\mathscr{F}}
\newcommand{\sG}{\mathscr{G}}
\newcommand{\sH}{\mathscr{H}}
\newcommand{\sI}{\mathscr{I}}
\newcommand{\sJ}{\mathscr{J}}
\newcommand{\sK}{\mathscr{K}}
\newcommand{\sL}{\mathscr{L}}
\newcommand{\sM}{\mathscr{M}}
\newcommand{\sN}{\mathscr{N}}
\newcommand{\sO}{\mathscr{O}}
\newcommand{\sP}{\mathscr{P}}
\newcommand{\sQ}{\mathscr{Q}}
\newcommand{\sR}{\mathscr{R}}
\newcommand{\sS}{\mathscr{S}}
\newcommand{\sT}{\mathscr{T}}
\newcommand{\sU}{\mathscr{U}}
\newcommand{\sV}{\mathscr{V}}
\newcommand{\sW}{\mathscr{W}}
\newcommand{\sX}{\mathscr{X}}
\newcommand{\sY}{\mathscr{Y}}
\newcommand{\sZ}{\mathscr{Z}}


\renewcommand{\emptyset}{\O}

\newcommand{\abs}[1]{\lvert #1 \rvert}
\newcommand{\norm}[1]{\lVert #1 \rVert}
\newcommand{\sm}{\setminus}


\newcommand{\sarr}{\rightarrow}
\newcommand{\arr}{\longrightarrow}

% NOTE: Defining collaborators is optional; to not list collaborators, comment out the line below.
%\newcommand{\collaborators}{Alyssa P. Hacker (\texttt{aphacker}), Ben Bitdiddle (\texttt{bitdiddle})}

\input{paolo-pset.tex}

% NOTE: To compile a version of this pset without problems, solutions, or reflections, uncomment the relevant line below.

%\excludeversion{problem}
%\excludeversion{solution}
%\excludeversion{reflection}

\begin{document}	
	
	% Use the \psetheader command at the beginning of a pset. 
	\psetheader
In this assignment, you may assume that holomorphic functions are infinitely differentiable. Moreover, if $O \subset \bbC$ is open, then for any $z\in \overline{D_r(z_0)}\subseteq O,$ 
\[f(z) = \sum_{n=0}^\infty \frac{f^{(n)}(z)}{n}(z - z_0)^n,\] where the series absolutely converges inside $D_r(z_0).$ 
\section*{Problem 1}
\begin{problem}
    Suppose $O\subset \bbC$ is open, $f: O \to \bbC$ and $f'(z_0)$ exists for some $z_0 \in O.$ If $z_0 = x_0 + iy_0$ and $u(x,y), v(x,y)$ are defined as the real and imaginary components of $f(z)$ respectively, then 
    \[\frac{\partial u}{\partial x}(x_0, y_0) = \frac{\partial v}{\partial y}(x_0, y_0), \quad \frac{\partial v}{\partial x}(x_0, y_0) = -\frac{\partial u}{\partial y}(x_0, y_0)\]
\end{problem}
\begin{solution}
Since $f$ is differentiable at $z_0,$ then it's partial's exist. 
    By the hint,
    \begin{align*}
f'(z_0) &= f'(x_0, y_0)\\
&= \lim_{h\to 0}\frac{[u(x_0 + h, y_0) + iv(x_0 + h, y_0)] - [u(x_0, y_0) - iv(x_0, y_0)]}{h}\\
&= \lim_{h\to 0}\frac{u(x_0 + h, y_0) - u(x_0, y_0)}{h} + i\lim_{h\to 0}\frac{v(x_0 + h, y_0) - v(x_0, y_0)}{h}\\
&= \frac{\partial u}{\partial x}(x_0, y_0) + i \frac{\partial v}{\partial x}(x_0, y_0)
    \end{align*}
and 
\begin{align*}
    f'(z_0) &= f'(x_0, y_0)\\
    &= \lim_{h\to 0}\frac{[u(x_0, y_0 + h) + iv(x_0, y_0 + h)] - [u(x_0, y_0) - iv(x_0, y_0)]}{ih}\\
    &= \frac{\partial v}{\partial y}(x_0, y_0)+ \frac{1}{i}\frac{\partial u}{\partial y}(x_0, y_0)\\
    &= \frac{\partial v}{\partial y}(x_0, y_0)- i\frac{\partial u}{\partial y}(x_0, y_0)
\end{align*}
Thus, we have that 
\[\Re{f'(z_0)} = \frac{\partial u}{\partial x}(z_0), \quad \Re{f'(z_0)} = \frac{\partial v}{\partial y}(z_0) \implies \frac{\partial u}{\partial x}(z_0) = \frac{\partial v}{\partial y}(z_0).\] Similarly, 
\[\frac{\partial v}{\partial x}(x_0, y_0)= -\frac{\partial u}{\partial y}(x_0, y_0)\]
\end{solution}

\newpage
\section*{Problem 2}
\begin{problem}
    Suppose $f \in H(O),$ where $O\subset \bbC$ is open. If $f: O \to \bbC.$ If $f(z) \in \bbR$ for all $z\in O,$ then $f$ is constant.
\end{problem}
\begin{solution}
Consider that for any $z\in O,$ $f(z) = u(z).$ Thus, $f = u$ and $v = 0.$
 By problem 3 on the previous PSET, it suffices to see that 
    \[\frac{\partial f}{\partial x} = \frac{\partial f}{\partial y} = 0.\] Note that since $f\in H(O),$ $f$ is differentiable for all of $O.$ By Problem 1 above, we have that for any $z\in O,$ 
    $\frac{\partial u}{\partial x} = \frac{\partial v}{\partial y}.$ But $v = 0,$ and thus $\frac{\partial u}{\partial x} = \frac{\partial v}{\partial y} = 0$ Similarly, $-\frac{\partial u}{\partial y} = \frac{\partial v}{\partial x} = 0.$ Thus, we are done, since all the partials are zero.
\end{solution}

\newpage
\section*{Problem 3}
\begin{problem}
    Suppose $f \in H(O).$ Prove that if $z\in O,$ then
    \[\nabla  u(z) = \nabla v(z) = 0.\]
\end{problem}
\begin{solution}
    We compute using Problem 1. Let $z\in O$ such that $z = x + iy.$ Then
    \begin{align*}
        \nabla  u(z)  &= \nabla u(x,y)\\
        &= \frac{\partial^2 u}{\partial x^2} + \frac{\partial ^2 u}{\partial y^2}\\
        &= \frac{\partial}{\partial x}(\frac{\partial u}{\partial x}) + \frac{\partial}{\partial y}(\frac{\partial u}{\partial y})\\
        &= \frac{\partial}{\partial x}(\frac{\partial v}{\partial y}) + \frac{\partial}{\partial y}(-\frac{\partial v}{\partial x})\\
        &= \frac{\partial}{\partial x}(\frac{\partial v}{\partial y}) - \frac{\partial}{\partial y}(\frac{\partial v}{\partial x})\\
        &= \frac{\partial^2 v}{\partial x \partial y} - \frac{\partial^2 v}{\partial y\partial x}\\
        \frac{\partial^2 v}{\partial x \partial y} - \frac{\partial^2 v}{\partial x\partial y}\\
        &= 0
    \end{align*}
    Similarly,
    \begin{align*}
        \nabla  v(z)  &= \nabla v(x,y)\\
        &= \frac{\partial^2 v}{\partial x^2} + \frac{\partial ^2 v}{\partial y^2}\\
        &= \frac{\partial}{\partial x}(\frac{\partial v}{\partial x}) + \frac{\partial}{\partial y}(\frac{\partial v}{\partial y})\\
        &= \frac{\partial}{\partial x}(-\frac{\partial u}{\partial y}) + \frac{\partial}{\partial y}(\frac{\partial u}{\partial x})\\
        &= -\frac{\partial}{\partial x}(\frac{\partial u}{\partial y}) + \frac{\partial}{\partial y}(\frac{\partial u}{\partial x})\\
        &=-\frac{\partial^2 u}{\partial x\partial y} + \frac{\partial^2 u}{\partial y\partial x}\\
        &= -\frac{\partial^2 u}{\partial x\partial y} + \frac{\partial^2 u}{\partial x\partial y}\\
        &= 0
    \end{align*}
Here, we use a few facts from multi-variable calculus. In particular, we use the fact that derivatives are linear and the Hessian matrix is symmetric.
\end{solution}

\newpage
\section*{Problem 4}
\begin{problem}
    Suppose $f \in H(O)$ where $O \subset \bbC$ is a connected open set. Suppose that for some $z_0 \in O,$ $f$ has a zero of infinite order. That is, $f^{(n)}(z_0) = 0$ for any $n\geq 0.$ Show that $f(z) = 0$ for any $z\in O.$
\end{problem}
\begin{solution}
Let 
\[A:= \{z \in O \mid f(z) = 0\}.\] We claim that $A \neq \emptyset,$ and that $A$ is clopen. 

Note that $A\neq \emptyset$ since $z_0 \in A$ since $f(z_0) = f^{(0)}(z_0) =0.$

Let $z'\in A.$ Since $O$ is open, there exists some $r>0$ such that $D_r(z')\subseteq O.$ Thus, $\overline{D_{\frac{r}{2}}(z')}\subset O.$ Let $z\in \overline{D_{\frac{r}{2}}(z')},$ then since $f\in H(O)$, 
\[f(z) = \sum_{n=0}^\infty \frac{f^{(n)}(z')}{n!}(z - z')^n = f(z') + f'(z')(z - z') + \frac{1}{2}f''(z')(z-z')^2 + \dots + \frac{1}{n!}f^{(n)}(z')(z - z')^n.\]
We know that since $z' \in A,$ then $f(z') = f'(z') = \dots = f^{(n)}(z') = 0,$ and thus $f(z) = 0.$ Then we have that $z \in A$ and so $A$ is open. 

Let $(z_n) \in A$ such that $z_n \to z.$ Since $z_n \in A,$ then $f(z_n) = 0$ for each $n.$ Since $f$ is differentiable, then it absolutely must be continuous, and so $f(z_n) \to f(z),$ and thus $f(z) = 0.$ We have showed that $A$ is closed.

Since $A$ is nonempty, open, and closed, and $O\supset A$ is connected, then $A = O.$\footnote{To see a proof of this, see previous PSET}. 
\end{solution}

\newpage
\section*{Problem 5}
\begin{problem}
    Suppose that we define 
    \[e^{z} = \sum_{n=0}^\infty \frac{z^n}{n!}, \quad \sin z = \sum_{n=0}^\infty \frac{z^{2n +1}}{(2n+1)!}(-1)^n, \quad \cos z = \sum_{n=0}^\infty \frac{z^{2n}}{(2n)!}(-1)^n, \quad \forall \; z\in \bbC.\] Prove that 
    \[e^{iz} = \cos z + i\sin z.\]
\end{problem}
\begin{solution}
 By definition, we compute:
 \begin{align*}
 e^{iz} &= \sum_{n=0}^\infty \frac{(iz)^n}{n!}\\
 &= 1 + iz - \frac{1}{2} z^2 - \frac{1}{3!}iz^3 + \frac{1}{4!}z^4 + \frac{1}{5!} iz^5 + \cdots\\
 &= (1 - \frac{1}{2}z^2 + \frac{1}{4!}z^4 - \frac{1}{6!}z^6 + \cdots) + (iz - \frac{1}{3!}iz^3 + \frac{1}{5!}iz^5+ \cdots)\\
 &= \sum_{n=0}^\infty \frac{(-1)^{n}}{(2n)!}z^{2n}  + i\sum_{n=0}^\infty \frac{(-1)^{n}}{(2n+1)!}z^{2n+1}\\
 &= \cos z + i\sin z
 \end{align*}
 
\end{solution}
\newpage
\section*{Problem 6}
\begin{problem}
    Suppose $O_1 \subseteq O_2,$ where $O_1$ is open in $\bbC$ and $O_2$ is open and connected in $\bbC.$ Suppose $f \in H(O).$ We say that $F \in H(O_2)$ is an \textbf{analytic continuation} of $f$ on $O_2$ if $F(z) = f(z)$ for any $z\in O_1.$ Prove that analytic continuations are unique. 
\end{problem}
\begin{solution}
    Let $F_1, F_2$ be analytic continuations of $f$ on $O_2.$ We want to show that $F_1 - F_2 = 0.$ Since $F_1, F_2 \in H(O),$ then we can take infinite derivatives of $F_1 - F_2.$ Consider that since $O_2 \subseteq \bbC$ is a connected open set, and if $z_0 \in O_1,$ then 
    \[F_1^{(n)}(z_0)- F_2^{(n)}(z_0)= f^{(n)}(z_0) - f^{(n)}(z_0) = 0, \quad \forall n \geq 0.\] Thus, by problem 4, we have that 
    \[(F_1 - F_2)(z) = 0, \quad \forall z\in O_2\] That is, $F_1(z) = F_2(z)$ for any $z\in O_2.$
\end{solution}

\newpage
\section*{Problem 7}
\begin{problem}
Assume that $f: O\to \bbC$ is continuous on an open connected set $O\subset \bbC$ such that 
\[\int_\gamma f(z)dz = 0\] for any closed path $\gamma$ on $O.$ Prove that $f$ is holomorphic on $O.$     
\end{problem}
\begin{solution}
\begin{lemma}
    Let $h \in \bbC.$ For any $z\in \bbC,$ we have that if $\gamma$ is the straight line from $z$ to $z + h,$ then 
    \[\int_\gamma d\zeta = h\]
\end{lemma}
\begin{proof}
    Clearly, $w$ is a primitive to $1$ since $w' = 1.$ Thus, we have that by the fundamental theorem of path integrals,
    \[\int_\gamma 1 d\zeta = \gamma(1) - \gamma(0) = z + h - z = h\]
\end{proof}
    Let $z_0 \in O.$  By the openness of $O,$ there exists some $r>0$ such that $\overline{D_r(z_0)}\subseteq O.$ We define $F: O\to \bbC$ as 
    \[F(z) = \int_{\gamma(z)} f(\zeta)d\zeta,\] where $\gamma$ is a path from from $z_0$ to $z.$ Indeed, such a path must exist since $O$ is connected and thus polygonally connected. 

To see that $F$ is well defined, let $\gamma$ and $\beta$ be two paths that start at $z_0$ and end at $z.$ Then $\gamma \circ \beta$ is a closed path starting from $z_0$ and ending $z_0.$ Thus, we have by assumption that
\[\int_{\gamma \circ \beta} f(z)dz = 0\] but 
\[\int_{\gamma \circ \beta} f(z)dz= \int_\gamma f(z)dz - \int_\beta f(z)dz  =0 \implies \int_\gamma f(z)dz =\int_\beta f(z)dz.\] Thus, $F$ is indeed well defined.

Moreover, we claim that if $\eta(t) = t(z+h) + (1-t)z$ is the straight path from $z$ to $z+h,$ then for small enough $h,$
\[F(z+h) - F(z) = \int_\eta f(\zeta)d\zeta.\] To see this, we can, by the path independence shown above, take $\gamma(z), \gamma(z + h)$ to be the polygonal paths. For $h< r,$ where $r>0$ such that the convex set $D_r(z)\subseteq O$ by openness, we can take $\eta$ to be the straight line from $z$ to $z +h.$ Thus, since $\gamma(z)\circ \eta$ is a path from $z_0$ to $z + h,$ then 
\[F(z+h) = F(z) + \int_\eta f(\zeta)d\zeta.\]
    
    
    We claim that on $O$ we have that $F'(z) = f(z).$ Let $\epsilon>0.$ Then since $f$ is continuous at $z$, then there exists some $\delta>0$ such that if $|z - \zeta| < \delta,$ then $|f(z) - f(\zeta)|< \epsilon.$ Take $h<\min\{\delta, r\},$ where $r>0$ such that $D_r(z)\subseteq O$ by the openness of $O.$ Then $\max_{\zeta \in [z, z+ h]}|f(\zeta) - f(z)| < \epsilon.$ Thus, since $\text{length}|\eta| = |h|,$ we have that
\begin{align*}
    \left|\frac{F(z + h) - F(z)}{h} - f(z)\right| &= \left| \frac{\int_{\gamma(z +h)}f(\zeta)d\zeta - \int_{\gamma(z)} f(\zeta)d\zeta}{h} - f(z)\right|\\
    &= \left| \frac{1}{h} \left[ \int_{z}^{z+h}f(\zeta)d\zeta - f(z)h \right]\right|\\
    &= \left|\frac{1}{h}\left[\int_z^{z + h}f(\zeta)d\zeta - f(z)\int_{z}^{z + h} d\zeta\right]\right|\\
    &= \left|\frac{1}{h}\int_z^{z + h}f(\zeta) - f(z)d\zeta\right|\\
    &\leq \max_{\zeta \in [z, z+ h]}|f(\zeta) - f(z)| |h|\\
    &< \frac{1}{|h|}\frac{\epsilon}{h} |h|\\
    &= \epsilon
\end{align*}

Since $F$ is differentiable in the disk, then it is infinitely differentiable. Since $f$ is one of those derivatives, then it also is infinitely differentiable. Thus, $f$ is holomorphic on this disk.
\end{solution}

\end{document}