\documentclass[11pt]{article}

% NOTE: Add in the relevant information to the commands below; or, if you'll be using the same information frequently, add these commands at the top of paolo-pset.tex file. 
\newcommand{\name}{AgustÃ­n Esteva}
\newcommand{\email}{aesteva@uchicago.edu}
\newcommand{\classnum}{20510}
\newcommand{\subject}{Accelerated Analysis in $\bbR^n$ III}
\newcommand{\instructors}{Don Stull}
\newcommand{\assignment}{Problem Set 8}
\newcommand{\semester}{Spring 2025}
\newcommand{\duedate}{05-21-2025}
\newcommand{\bA}{\mathbf{A}}
\newcommand{\bB}{\mathbf{B}}
\newcommand{\bC}{\mathbf{C}}
\newcommand{\bD}{\mathbf{D}}
\newcommand{\bE}{\mathbf{E}}
\newcommand{\bF}{\mathbf{F}}
\newcommand{\bG}{\mathbf{G}}
\newcommand{\bH}{\mathbf{H}}
\newcommand{\bI}{\mathbf{I}}
\newcommand{\bJ}{\mathbf{J}}
\newcommand{\bK}{\mathbf{K}}
\newcommand{\bL}{\mathbf{L}}
\newcommand{\bM}{\mathbf{M}}
\newcommand{\bN}{\mathbf{N}}
\newcommand{\bO}{\mathbf{O}}
\newcommand{\bP}{\mathbf{P}}
\newcommand{\bQ}{\mathbf{Q}}
\newcommand{\bR}{\mathbf{R}}
\newcommand{\bS}{\mathbf{S}}
\newcommand{\bT}{\mathbf{T}}
\newcommand{\bU}{\mathbf{U}}
\newcommand{\bV}{\mathbf{V}}
\newcommand{\bW}{\mathbf{W}}
\newcommand{\bX}{\mathbf{X}}
\newcommand{\bY}{\mathbf{Y}}
\newcommand{\bZ}{\mathbf{Z}}
\newcommand{\Vol}{\text{Vol}}

%% blackboard bold math capitals
\newcommand{\bbA}{\mathbb{A}}
\newcommand{\bbB}{\mathbb{B}}
\newcommand{\bbC}{\mathbb{C}}
\newcommand{\bbD}{\mathbb{D}}
\newcommand{\bbE}{\mathbb{E}}
\newcommand{\bbF}{\mathbb{F}}
\newcommand{\bbG}{\mathbb{G}}
\newcommand{\bbH}{\mathbb{H}}
\newcommand{\bbI}{\mathbb{I}}
\newcommand{\bbJ}{\mathbb{J}}
\newcommand{\bbK}{\mathbb{K}}
\newcommand{\bbL}{\mathbb{L}}
\newcommand{\bbM}{\mathbb{M}}
\newcommand{\bbN}{\mathbb{N}}
\newcommand{\bbO}{\mathbb{O}}
\newcommand{\bbP}{\mathbb{P}}
\newcommand{\bbQ}{\mathbb{Q}}
\newcommand{\bbR}{\mathbb{R}}
\newcommand{\bbS}{\mathbb{S}}
\newcommand{\bbT}{\mathbb{T}}
\newcommand{\bbU}{\mathbb{U}}
\newcommand{\bbV}{\mathbb{V}}
\newcommand{\bbW}{\mathbb{W}}
\newcommand{\bbX}{\mathbb{X}}
\newcommand{\bbY}{\mathbb{Y}}
\newcommand{\bbZ}{\mathbb{Z}}

%% script math capitals
\newcommand{\sA}{\mathscr{A}}
\newcommand{\sB}{\mathscr{B}}
\newcommand{\sC}{\mathscr{C}}
\newcommand{\sD}{\mathscr{D}}
\newcommand{\sE}{\mathscr{E}}
\newcommand{\sF}{\mathscr{F}}
\newcommand{\sG}{\mathscr{G}}
\newcommand{\sH}{\mathscr{H}}
\newcommand{\sI}{\mathscr{I}}
\newcommand{\sJ}{\mathscr{J}}
\newcommand{\sK}{\mathscr{K}}
\newcommand{\sL}{\mathscr{L}}
\newcommand{\sM}{\mathscr{M}}
\newcommand{\sN}{\mathscr{N}}
\newcommand{\sO}{\mathscr{O}}
\newcommand{\sP}{\mathscr{P}}
\newcommand{\sQ}{\mathscr{Q}}
\newcommand{\sR}{\mathscr{R}}
\newcommand{\sS}{\mathscr{S}}
\newcommand{\sT}{\mathscr{T}}
\newcommand{\sU}{\mathscr{U}}
\newcommand{\sV}{\mathscr{V}}
\newcommand{\sW}{\mathscr{W}}
\newcommand{\sX}{\mathscr{X}}
\newcommand{\sY}{\mathscr{Y}}
\newcommand{\sZ}{\mathscr{Z}}


\renewcommand{\emptyset}{\O}

\newcommand{\abs}[1]{\lvert #1 \rvert}
\newcommand{\norm}[1]{\lVert #1 \rVert}
\newcommand{\sm}{\setminus}


\newcommand{\sarr}{\rightarrow}
\newcommand{\arr}{\longrightarrow}

% NOTE: Defining collaborators is optional; to not list collaborators, comment out the line below.
%\newcommand{\collaborators}{Alyssa P. Hacker (\texttt{aphacker}), Ben Bitdiddle (\texttt{bitdiddle})}

\input{paolo-pset.tex}

% NOTE: To compile a version of this pset without problems, solutions, or reflections, uncomment the relevant line below.

%\excludeversion{problem}
%\excludeversion{solution}
%\excludeversion{reflection}

\begin{document}	
	
	% Use the \psetheader command at the beginning of a pset. 
	\psetheader
    
    
    \section*{Problem 1}
Which of the following forms on $\mathbb{R}^3$ are closed?
\begin{enumerate}
    \item $\omega = x \, dx \wedge dy \wedge dz$
    \begin{solution}
    \begin{align*}
        d\omega &= d\left(x \, dx \wedge dy \wedge dz\right)\\
        &= \left(\frac{\partial}{\partial x}x\,dx + \frac{\partial}{\partial y}x\,dy + \frac{\partial}{\partial z}x\,dz\right)\wedge dx \wedge dy \wedge dz\\
        &= 1\,dx \wedge\,dx \wedge dy \wedge dz\\
        &= (dx\wedge dx) \wedge dy \wedge dz\\
        &= 0
    \end{align*}
    \end{solution}
    \item $\omega = z \, dy \wedge dx + x \, dy \wedge dz$
\begin{solution}
        \begin{align*}
        d\omega &= d\left(z \, dy \wedge dx + x \, dy \wedge dz\right)\\
        &= d\left(z \, dy \wedge dx\right) + d\left(x\,  dy \wedge dz\right)\\
        &= \left(\frac{\partial}{\partial x}z\,dx + \frac{\partial}{\partial y}z\,dy + \frac{\partial}{\partial z}z\,dz\right)\wedge dy \wedge dx + \left(\frac{\partial}{\partial x}x\,dx + \frac{\partial}{\partial y}x\,dy + \frac{\partial}{\partial z}x\,dz\right)\wedge dy\wedge dz\\
        &= dz\wedge dy\wedge dx + dx \wedge dy \wedge dz\\
        &= (-1)^3 \,dx\wedge dy\wedge dz+ dx\wedge dy\wedge dz\\
        &= 0
    \end{align*}
\end{solution}
    \item $\omega = x \, dx + y \, dy$
\begin{solution}
    \begin{align*}
        d\omega &= d\left( x\,dx\right)  + d(y\,dy)\\
        &= \left(\frac{\partial}{\partial x}x\,dx + \frac{\partial}{\partial y}x\,dy + \frac{\partial}{\partial z}x\,dz\right)\wedge dx + \left(\frac{\partial}{\partial x}y\,dx + \frac{\partial}{\partial y}y\,dy + \frac{\partial}{\partial z}y\,dz\right)\wedge dy\\
        &= dx\wedge dx + dy\wedge dy\\
        &= 0
    \end{align*}
\end{solution}
\end{enumerate}



\newpage
\section*{Problem 2}
Show that every $k$-form on $\mathbb{R}^k$ is closed.
\begin{solution}
    Consider first the case when 
    \[\omega = f \,dx_1\wedge \cdots dx_k,\] Then
    \begin{align*}
        d\omega &= \left(\sum_{i=1}^k \frac{\partial f}{\partial x_i}\wedge dx_i\right) \wedge dx_1 \cdots \wedge dx_k\\
        &= \sum_{i=1}^k \left(\frac{\partial f}{\partial x_i}\wedge dx_i \wedge dx_1 \cdots \wedge dx_k\right)\\
        &= \sum_{i=1}^k 0
    \end{align*}
    by the repeated index in every sum. Now consider 
    \[\omega = f\,dx_{i_1}\wedge \cdots \wedge dx_{i_k} = (-1)^\alpha f \,dx_1 \wedge \cdots \wedge dx_k,\] we get that by the first case, since $(-1)^\alpha$ is a constant\footnote{Let $\omega$ be a $k-$form and $c>0$, then $d(c\omega) = cd(\omega)$. To see this, note that we can pull out the $c$ constant out of every partial in the sum}
    \[d\omega = (-1)^\alpha d\left(f \,dx_1 \wedge \cdots \wedge dx_k\right) = (-1)^\alpha (0) = 0\]
    For the general case, let 
    \[\omega = \sum_I f_I \,dx_I,\] where the $I = \sigma\{1,2,\dots, k\}$ are permutations of $\{1,2,\dots, k\}.$ Then by definition,
    \[d \omega = \sum_I (df_I)\wedge dx_I = \sum_I 0 = 0\]

\end{solution}

\newpage
\section*{Problem 3}
In $\mathbb{R}^4$, consider the following 2-form 
\[ \omega = dx_1 \wedge dx_2 + dx_3 \wedge dx_4. \]
Compute $\omega \wedge \omega$ and $\omega \wedge \omega \wedge \omega$. Find a 1-form $\eta$ such that $d\eta = \omega$. This 1-form is called the Liouville form.
\begin{solution}
    \begin{align*}
        \omega\wedge \omega &= (dx_1 \wedge dx_2 + dx_3 \wedge dx_4) \wedge(dx_1 \wedge dx_2 + dx_3 \wedge dx_4) \\
        &= (dx_1 \wedge dx_2)\wedge (dx_1 \wedge dx_2) + 2\,(dx_1 \wedge dx_2)\wedge (dx_3 \wedge dx_4)+ (dx_3 \wedge dx_4)\wedge (dx_3 \wedge dx_4)\\
        &= 2 \,dx_1 \wedge dx_2 \wedge dx_3 \wedge dx_4
    \end{align*}
    Using this, 
    \begin{align*}
        \omega \wedge \omega \wedge \omega &= (\omega \wedge \omega) \wedge \omega\\
        &= (2 \,dx_1 \wedge dx_2 \wedge dx_3 \wedge dx_4) \wedge (dx_1 \wedge dx_2 + dx_3 \wedge dx_4)\\
        &= 2(dx_1 \wedge dx_2) \wedge dx_3 \wedge dx_4 \wedge (dx_1 \wedge dx_2) + 2\,dx_1 \wedge dx_2 \wedge (dx_3 \wedge dx_4) \wedge (dx_3 \wedge dx_4)\\
        &= 0 + 0\\
        &= 0
    \end{align*}
    Consider 
    \[\eta = x_1 \,dx_2 + x_3 \, dx_4.\]
    Then 
    \begin{align*}
        d\eta &= \left(\frac{\partial }{\partial x_1}x_1 dx_1 +   \frac{\partial }{\partial x_1}x_1 dx_2 + \frac{\partial }{\partial x_1}x_1 dx_3 + \frac{\partial }{\partial x_1}x_1 dx_4\right)\wedge dx_2\\
        \qquad &+ \left(\frac{\partial }{\partial x_1}x_3 dx_1 +   \frac{\partial }{\partial x_2}x_3 dx_2 + \frac{\partial }{\partial x_3}x_3 dx_3 + \frac{\partial }{\partial x_4}x_3 dx_4\right)\wedge dx_4\\
        &= dx_1 \wedge dx_w + dx_3 \wedge dx_4
    \end{align*}
\end{solution}

\newpage
\section*{Problem 4}
\begin{problem}
    Suppose $\sigma = [p_0, \dots, p_k]$ is an oriented affine $k-$simplex. Show that $\partial^2 \sigma = 0.$
\end{problem}
\begin{solution}
    Let \[\sigma_i = [p_0, \dots, p_{i-1}, p_{i+1}, \dots, p_k]\] and \[\sigma_{ij} = [p_0, \dots, p_{j-1}, p_{j+1}, \dots, p_{i-1}, p_{i+1}, \dots, p_k].\] That is, $\sigma_{ij}$ is the oriented affine $k-2$simplex with the $i$ and $j$ coordinate removed. Without loss of generality up to a sign, suppose $k$ is odd. Then by definition 
    \begin{align*}
        \partial \sigma = \sigma_0 - \sigma_1 + \dots - \sigma_k.
    \end{align*}
    Since $\partial\sigma$ is a oriented affine $k-1$ chain, then by definition
    \begin{align*}
        \partial(\partial \sigma) &= \partial\sigma_0 - \partial\sigma_1 + \dots - \partial \sigma_k\\
        &= (\sigma_{01} - \sigma_{02} + \dots +\sigma_{0k})- (\sigma_{10} - \sigma_{12} + \dots + \sigma_{1k}) + \dots -(\sigma_{k0} - \sigma_{k1} + \cdots + \sigma_{k(k-1)})
    \end{align*}
    It is clear that for any $i, j$ where $i\neq j,$ $\sigma_{ij} = \sigma_{ji}.$ Thus, we see that the sum above is zero.
\end{solution}

\newpage
\section*{Problem 5}
\begin{problem}
    Define $J^2 = \tau_1 + \tau_2,$ where
    \[\tau_1 = [\textbf{0}, e_1, e_1 + e_2] \qquad \tau_2 = -[\textbf{0}, e_2, e_2 + e_1].\] Explain why it is reasonable to call $J^2$ the positively oriented unit square in $\bbR^2.$ What is $\partial J^2?$ 
\end{problem}
\begin{solution}
    We know that $\tau_1$ is the triangle with edges $(0,0), (1,0), (1,1)$ with the orientation that 
    \[(0,0)\to (1,0)\to (1,1)\to (0,0).\] Meanwhile, $\tau_2$ is the triangle with edges $(0,0), (0,1), (1,1)$ such that 
    \[(0,0)\leftarrow(0,1)\leftarrow(1,1)\leftarrow(0,0).\] Thus, the diagonal lines 'cancel out' and we are left with the unit square. By definition, 
    \begin{align*}
        \partial J^2 &= \partial \tau_1 + \partial \tau _2\\ &= ([e_1, e_1 + e_2] - [0, e_1 + e_2] + [0, e_1]) - ([e_2, e_2 + e_1]- [0, e_2 + e_1] + [0, e_2])\\
        &= [e_1, e_1 + e_2] +[0, e_1] - [e_2, e_2 + e_1] - [0,e_2]
    \end{align*}
\end{solution}


\newpage
\begin{problem}
    Consider the oriented affine $3-$simplex
    \[\sigma_1 = [0, e_1, e_1 + e_2, e_1 + e_2 + e_3]\] has determinant $1$ when regarded as a linear transform and is thus positively oriented.
\end{problem}
\begin{solution}
    $\sigma_1$ when regarded as a linear transform is simply the identity mapping and therefore has determinant $1.$ 
\end{solution}

\newpage
\section*{Problem 6}
\begin{problem}
    State the conditions under which the formula 
    \[\int_\Phi f\,d\omega = \int_{d\Phi}f \,\omega - \int_{\Phi}(df)\wedge \omega\]
\end{problem}
\begin{solution}
Let $E \subseteq \bbR^n$ be open and $F\subseteq \bbR^m$ be open. Let $f\in C^1(E, \bbR)$ and $\omega \in \Lambda^{k-1}(F)$ be of class $C^1.$ Suppose $\Phi\in C^2(E,F)$ is a $k-$chain. Since $f\omega = f\wedge \omega \in \Lambda^{k-1}(F),$ then we apply Stokes' theorem to find that 
\[\int_{\partial\Phi} f\omega = \int_{\Phi} d(f\omega) = \int_{\Phi} (df \wedge \omega + f \wedge d\omega) = \int_\Phi df\wedge \omega + \int_{\Phi} f\wedge d\omega,\] and so the conclusion follows from subtracting. Recall the integration by parts formula. Let $f,g \in C^1([a,b], \bbR),$ then 
\[\int_a^b (f'g)(x) \,dx= [(fg)(b) - (fg)(a)] - \int_a^b (fg')(x)\,dx.\] Letting $\Phi = [a,b]$ be the oriented $1-$simplex, we have that $\partial \Phi = [b] - [a].$ Letting $\omega = g,$ we see that 
\[d\omega = g'\qquad df = f'.\] Thus, 
\[\int_{\partial \Phi} fg = \int_{[b] - [a]}fg = \int_{[b]}fg - \int_{[a]}fg = (fg)(b) - (fg)(b).\] Letting $\Delta:[a,b]\to [a,b]$ be the identity, we use the definition of the integral over forms to see that 
\[\int_{\Phi}f\,d\omega = \int_{[a,b]}fg' = \int_{\Delta([a,b])}fg' = \int_a^b (fg')(\Delta(x))\Delta'(x)\,dx = \int_a^b (fg')(x)\,dx.\] Similarly, 
\[\int_{\Phi}(df)\wedge \omega = \int_a^b f'g.\] Thus, we have recovered the integration by parts formula.
\end{solution}

\newpage
\section*{Problem 7}
\begin{problem}
    Define the annulus to be the $2-$surface 
    \[\Phi(r,\theta) = (r\cos \theta, r\sin \theta)\qquad a\leq r\leq b, \theta \in [0,2\pi].\]Let $\omega = x^3\,dy.$ Show that Stokes theorem holds by computing both sides explicitly.
\end{problem}
\begin{solution}
Note that by the standard change of variables, 
\[\int_{\Phi}d\omega = \int_{[a,b]\times [0,2\pi]}(d\omega)_\Phi.\] 
We have that 
    \[d\omega = 3x^2\,dx \wedge dy.\] 
Pulling back, 
\[dt_1 = \cos \theta \,dr -r\sin\theta\,d\theta\]
\[dt_2 = \sin\theta\,dr + r\cos\theta\,d\theta\] and thus 
\begin{align*}
    (d\omega)_\Phi &= 3x^2(T(x_1))\,dt_1 \wedge dt_2\\
    &= 3r^2\cos^2\theta \left[(\cos \theta \,dr -r\sin\theta\,d\theta) \wedge (\sin\theta\,dr + r\cos\theta\,d\theta)\right]\\
    &= 3r^2\cos^2\theta[r\cos^2\theta\,dr\wedge d\theta - r\sin^2\theta\,d\theta \wedge dr]\\
    &= 3r^3\cos^2 \theta \,dr\wedge d\theta
\end{align*}
Thus, 
\begin{align*}
\int_{\Phi}d\omega &= \int_{\Delta([a,b]\times [0,2\pi])}3r^3\cos^2 \theta \,dr\wedge d\theta\\ &= \int_0^{2\pi}\int_a^b 3(\Delta_r(u))^3 \cos^2(\Delta_\theta(u)\, \Delta'(u)\,du\\ &= \int_0^{2\pi}\int_a^b 3r^4 \cos^2(\theta)\,dr\,d\theta   \\
&= \int_0^{2\pi} \frac{3}{4}(b^4 - a^4)\cos^2\theta \,d\theta\\
&= \frac{3\pi}{4}(b^4 - a^4)
\end{align*}
On the other hand, since $\Phi = T\circ J^2,$ where $T(r,\theta) = (r\sin\theta, r\cos \theta)$ and $J^2= \tau_1 + \tau_2, $ where 
\[\tau_1 = [(a,0), (b,0), (b, 2\pi)]\qquad \tau = -[(a,0), (0,2\pi), (b, 2\pi)].\] We've computed that 
\[\partial J^2 = [(b,0), (b, 2\pi)] + [(a,0), (b, 0)] - [(a,2\pi), (b, 2\pi)] - [(a,0), (a,2\pi)]\] and so 
\[T\circ \partial J^2 = [b\sin\theta, b\cos \theta] + [0, r] - [0, r] - [a\sin\theta, a\cos\theta].\] Define $R(\theta)= (b\sin\theta, b\cos\theta)$ and $S(\theta) = (a\sin\theta, a\cos \theta).$
\begin{align*}
    \int_{\partial \Phi} \omega &= \int_{[b\sin\theta, b\cos \theta]}x^3\,dy - \int_{[a\sin\theta, a\cos\theta]}x^3\,dy\\
    &= \int_{R[0,2\pi]} x^3\,dy - \int_{S[0,2\pi]}x^3 \,dy\\
    &= \int_{\Delta[0,2\pi]} (x^3\,dy)_R - \int_{\Delta[0,2\pi]}(x^3\,dy)_S\\
    &= \int_{\Delta[0,2\pi]} (-b^4 \sin^4\theta)\,d\theta - \int_{\Delta[0,2\pi]}(-a^4\sin^4 \theta)\,d\theta\\
    &= (a^4 - b^4)\int_0^{2\pi}\sin^4\theta\,d\theta\\
    &= (a^4 - b^4)\frac{3\pi }{4}
\end{align*}

\end{solution}

\end{document}